pneutube

test/artifact/hacl-star/pneutube/tube.c
@@ -13,7 +13,7 @@
 #include <errno.h>
 #include <arpa/inet.h>
 #include "FStar_IO.h"
-#include "Hacl_Tube.h"
+#include "Hacl_Tube_Receive.h"
 
 #define secretbox_MACBYTES   16
 #define secretbox_NONCEBYTES 24
@@ -125,10 +125,10 @@ int main(int argc, char *argv[]){
   if (argc - optind == 3 && strcmp(argv[optind], "send") == 0) {
       strcpy(file, argv[optind+1]);
       sscanf(argv[optind+2],"%512[^:]:%u",host,&port);
-      Hacl_Tube_file_send(strlen(file),file,roundup,host,port,sk,pk);
+      Hacl_Tube_Send_file_send(strlen(file),file,roundup,host,port,sk,pk);
   } else if (argc - optind == 2 && strcmp(argv[optind], "receive") == 0) {
       sscanf(argv[optind+1],"%u",&port);
-      Hacl_Tube_file_recv(port,pk,sk);
+      Hacl_Tube_Receive_file_recv(port,pk,sk);
   } else {
     print_usage();
     abort();
